Save progress

hpaxos.thy
@@ -82,33 +82,50 @@ axiomatization where
 (*
 Morally, messages have the following inductive structure
 
-T1a : \<forall> n: nat. Ballot \<Rightarrow> MessageRec n
-T1b : \<forall> n: nat. Acceptor \<Rightarrow> FINSUBSET(MessageRec n, MessageDepthRange) \<Rightarrow> MessageRec (n + 1)
-T2a : \<forall> n: nat. Learner \<Rightarrow> Acceptor \<Rightarrow> FINSUBSET(MessageRec n, MessageDepthRange) \<Rightarrow> MessageRec (n + 1)
+M1a : \<forall> n: nat. Ballot \<Rightarrow> MessageRec n
+M1b : \<forall> n: nat. Acceptor \<Rightarrow> FINSUBSET(MessageRec n, MessageDepthRange) \<Rightarrow> MessageRec (n + 1)
+M2a : \<forall> n: nat. Learner \<Rightarrow> Acceptor \<Rightarrow> FINSUBSET(MessageRec n, MessageDepthRange) \<Rightarrow> MessageRec (n + 1)
 
 Message \<equiv> \<Union>n. {MessageRec n}
 *)
 
 datatype PreMessage = 
-  T1a Ballot 
-| T1b "Acceptor * PreMessage list" 
-| T2a "Learner * Acceptor * PreMessage list"
+  M1a Ballot 
+| M1b Acceptor "PreMessage list" 
+| M2a Learner Acceptor "PreMessage list"
 
 fun isValidMessage :: "PreMessage \<Rightarrow> bool" where
-  "isValidMessage (T1a _) = True" |
-  "isValidMessage (T1b (_, msgs)) = (msgs \<noteq> [] \<and> length msgs \<le> MaxRefCardinality \<and> list_all isValidMessage msgs)" |
-  "isValidMessage (T2a (_, _, msgs)) = (msgs \<noteq> [] \<and> length msgs \<le> MaxRefCardinality \<and> list_all isValidMessage msgs)"
+  "isValidMessage (M1a _) = True" |
+  "isValidMessage (M1b _ msgs) = (msgs \<noteq> [] \<and> length msgs \<le> MaxRefCardinality \<and> list_all isValidMessage msgs)" |
+  "isValidMessage (M2a _ _ msgs) = (msgs \<noteq> [] \<and> length msgs \<le> MaxRefCardinality \<and> list_all isValidMessage msgs)"
 
 typedef (overloaded) Message = "{a::PreMessage. isValidMessage a}"
 proof
-  show "T1a 0 \<in> {a::PreMessage. isValidMessage a}"
+  show "M1a 0 \<in> {a::PreMessage. isValidMessage a}"
     by simp
 qed
 
+datatype MessageType = T1a | T1b | T2a
+
+fun type :: "PreMessage \<Rightarrow> MessageType" where
+  "type (M1a _) = T1a" |
+  "type (M1b _ msgs) = T1b" |
+  "type (M2a _ _ msgs) = T2a"
+
 fun ref :: "PreMessage \<Rightarrow> PreMessage set" where
-  "ref (T1a _) = {}" |
-  "ref (T1b (_, msgs)) = set msgs" |
-  "ref (T2a (_, _, msgs)) = set msgs"  
+  "ref (M1a _) = {}" |
+  "ref (M1b _ msgs) = set msgs" |
+  "ref (M2a _ _ msgs) = set msgs"  
+
+fun acc :: "PreMessage \<Rightarrow> Acceptor" where
+  "acc (M1a _) = undefined" |
+  "acc (M1b a _) = a" |
+  "acc (M2a _ a _) = a"
+
+fun lrn :: "PreMessage \<Rightarrow> Learner" where
+  "lrn (M1a _) = undefined" |
+  "lrn (M1b _ _) = undefined" |
+  "lrn (M2a l _ _) = l"
 
 (* Transitive references *)
 (* ------------------------------------------------------------------- *)
@@ -116,18 +133,182 @@ fun ref :: "PreMessage \<Rightarrow> PreMessage set" where
 (*If we always want TranDepthRange to be finite, we can simply do*)
 fun TranF :: "nat \<Rightarrow> PreMessage \<Rightarrow> PreMessage set" where
   "TranF 0 m = {m}" |
-  "TranF n (T1a a) = {T1a a}" |
-  "TranF n (T1b (a, msgs)) = {T1b (a, msgs)} \<union> \<Union> (TranF (n-1) ` set msgs)" |
-  "TranF n (T2a (a, l, msgs)) = {T2a (a, l, msgs)} \<union> \<Union> (TranF (n-1) ` set msgs)"  
+  "TranF n (M1a a) = {M1a a}" |
+  "TranF n (M1b a msgs) = {M1b a msgs} \<union> \<Union> (TranF (n-1) ` set msgs)" |
+  "TranF n (M2a a l msgs) = {M2a a l msgs} \<union> \<Union> (TranF (n-1) ` set msgs)"  
 
 (* This is Tran as it actually is in the original file *)
 fun Tran :: "PreMessage \<Rightarrow> PreMessage set" where
-  "Tran (T1a a) = {T1a a}" |
-  "Tran (T1b (a, msgs)) = {T1b (a, msgs)} \<union> \<Union> (Tran ` set msgs)" |
-  "Tran (T2a (a, l, msgs)) = {T2a (a, l, msgs)} \<union> \<Union> (Tran ` set msgs)"  
+  "Tran (M1a a) = {M1a a}" |
+  "Tran (M1b a msgs) = {M1b a msgs} \<union> \<Union> (Tran ` set msgs)" |
+  "Tran (M2a a l msgs) = {M2a a l msgs} \<union> \<Union> (Tran ` set msgs)"  
+
+theorem Valid_contains_ballot:
+  assumes "isValidMessage m"
+  shows "\<exists>a. M1a a \<in> Tran m"
+using assms
+proof (induction m)
+  case (M1a a)
+  then show ?case by simp
+next
+  case (M1b a msgs)
+  then show ?case
+    by (metis Ball_set Tran.simps(2) UN_I UnCI isValidMessage.simps(2) last_in_set)
+next
+  case (M2a a l msgs)
+  then show ?case
+    by (metis Ball_set Tran.simps(3) UN_I UnCI isValidMessage.simps(3) last_in_set)
+qed
 
 (* Algorithm specification *)
 (* ------------------------------------------------------------------- *)
+
+(*
+A bit different than the original.
+The original returned the singleton set containing
+The largest Ballot. Here, we just return the largest Ballot
+
+Note that, in the case that a PreMessage isn't valid,
+this may be in error as Max may be called on an empty set.
+*)
+fun Get1a :: "PreMessage \<Rightarrow> Ballot" where
+  "Get1a m = Max {a . M1a a \<in> Tran m}"
+
+fun B :: "PreMessage \<Rightarrow> Ballot \<Rightarrow> bool" where
+  "B m bal = (bal = Get1a m)"
+
+record State =
+  msgs :: "PreMessage list"
+  known_msgs_acc :: "Acceptor \<Rightarrow> PreMessage list"
+  known_msgs_lrn :: "Learner \<Rightarrow> PreMessage list"
+  recent_msgs_acc :: "Acceptor \<Rightarrow> PreMessage list"
+  recent_msgs_lrn :: "Learner \<Rightarrow> PreMessage list"
+  queued_msg :: "Acceptor \<Rightarrow> PreMessage option"
+  two_a_lrn_loop :: "Acceptor \<Rightarrow> bool"
+  processed_lrns :: "Acceptor \<Rightarrow> Learner list"
+  decision :: "Learner \<Rightarrow> Ballot \<Rightarrow> Value list"
+  BVal :: "Ballot \<Rightarrow> Value"
+
+definition NoMessage :: "PreMessage option" where
+  "NoMessage = None"
+
+fun Init :: "(Ballot \<Rightarrow> Value) \<Rightarrow> State" where
+  "Init bval = \<lparr> 
+      msgs = [], 
+      known_msgs_acc = (\<lambda>_. []), 
+      known_msgs_lrn = (\<lambda>_. []), 
+      recent_msgs_acc = (\<lambda>_. []), 
+      recent_msgs_lrn = (\<lambda>_. []), 
+      queued_msg = (\<lambda>_. NoMessage), 
+      two_a_lrn_loop = (\<lambda>_. False), 
+      processed_lrns = (\<lambda>_. []), 
+      decision = (\<lambda>_ _. []), 
+      BVal = bval 
+    \<rparr>"
+
+fun V :: "State \<Rightarrow> PreMessage \<Rightarrow> Value \<Rightarrow> bool" where
+  "V st m val = (val = BVal st (Get1a m))"
+
+(*Maximal ballot number of any messages known to acceptor a*)
+(* Direct translation *)
+fun MaxBalL :: "State \<Rightarrow> Acceptor \<Rightarrow> Ballot \<Rightarrow> bool" where
+  "MaxBalL st a mbal = 
+      ((\<exists> m \<in> set (known_msgs_acc st a). B m mbal)
+      \<and> (\<forall> x \<in> set (known_msgs_acc st a).
+          \<forall> b :: Ballot. B x b \<longrightarrow> b \<le> mbal))"
+
+(*Better implementation*)
+fun MaxBalO :: "State \<Rightarrow> Acceptor \<Rightarrow> Ballot option" where
+  "MaxBalO st a = 
+    (if known_msgs_acc st a = [] then None else
+     Some (Max (Get1a ` set (known_msgs_acc st a))))"
+
+fun MaxBal :: "State \<Rightarrow> Acceptor \<Rightarrow> Ballot \<Rightarrow> bool" where
+  "MaxBal st a mbal = (Some mbal = MaxBalO st a)"
+
+fun SameBallot :: "PreMessage \<Rightarrow> PreMessage \<Rightarrow> bool" where
+  "SameBallot x y = (\<forall> b. B x b = B y b)"
+
+(*
+The acceptor is _caught_ in a message x if the transitive references of x
+include evidence such as two messages both signed by the acceptor, in which
+neither is featured in the other's transitive references.
+*)
+fun CaughtMsg :: "PreMessage \<Rightarrow> PreMessage set" where
+  "CaughtMsg x = 
+    { m . m \<in> Tran x 
+        \<and> type m \<noteq> T1a
+        \<and> (\<exists> m1 \<in> Tran x.
+              type m1 \<noteq> T1a
+           \<and> acc m = acc m1
+           \<and> m \<notin> Tran m1
+           \<and> m1 \<notin> Tran m
+        ) }"
+
+fun Caught :: "PreMessage \<Rightarrow> Acceptor set" where
+  "Caught x = acc ` { m . m \<in> CaughtMsg x }"
+
+fun ConByQuorum :: "Learner \<Rightarrow> Learner \<Rightarrow> PreMessage \<Rightarrow> (Acceptor \<Rightarrow> bool) \<Rightarrow> bool" where
+  "ConByQuorum a b x S = (
+      TrustSafe a b S \<and> 
+      (\<forall> a \<in> Caught x. \<not> (S a))
+    )"
+
+fun Con :: "Learner \<Rightarrow> PreMessage \<Rightarrow> Learner set" where
+  "Con a x = {b . \<exists> S. is_quorum S \<and> ConByQuorum a b x S}"
+
+(*
+2a-message is _buried_ if there exists a quorum of acceptors that have seen
+2a-messages with different values, the same learner, and higher ballot
+numbers.
+*)
+fun Buried :: "State \<Rightarrow> PreMessage \<Rightarrow> PreMessage \<Rightarrow> bool" where
+  "Buried st x y = 
+    (let Q :: PreMessage set = 
+      { m. m \<in> Tran y 
+          \<and> (\<exists>z \<in> Tran m.
+                  type z = T2a
+                \<and> lrn z = lrn x
+                \<and> (\<forall> bx bz :: Ballot.
+                      B x bx \<and> B z bz \<longrightarrow> bx < bz
+                  )
+                \<and> (\<forall> vx vz :: Value.
+                      V st x vx \<and> V st z vz \<longrightarrow> vx \<noteq> vz
+                  )
+            ) }
+     in TrustLive (lrn x) (\<lambda>a . a \<in> acc ` Q)
+    )
+  "
+
+(* Connected 2a messages *)
+fun Con2as :: "State \<Rightarrow> Learner \<Rightarrow> PreMessage \<Rightarrow> PreMessage set" where
+  "Con2as st l x = 
+    { m . m \<in> Tran x
+        \<and> type m = T2a
+        \<and> acc m = acc x
+        \<and> \<not> (Buried st m x)
+        \<and> lrn m \<in> Con l x
+    }"
+
+(*Fresh 1b messages*)
+fun Fresh :: "State \<Rightarrow> Learner \<Rightarrow> PreMessage \<Rightarrow> bool" where
+  "Fresh st l x =
+    (\<forall>m \<in> Con2as st l x. \<forall>v :: Value. V st x v = V st m v)
+  "
+
+(* Quorum of messages referenced by 2a *)
+fun q :: "State \<Rightarrow> PreMessage \<Rightarrow> Acceptor set" where
+  "q st x = (
+    let Q = { m . m \<in> Tran x
+                \<and> type m = T1b
+                \<and> Fresh st (lrn x) m
+                \<and> (\<forall>b :: Ballot. B m b = B x b)
+            }
+    in acc ` Q
+  )"
+
+
+
 
 
 (*
